\documentclass[a0paper,landscape,fleqn]{article}
\usepackage[margin=1cm]{geometry}
\usepackage[utf8]{inputenc}
\usepackage[T1]{fontenc}
\usepackage{amsfonts,amssymb}
\usepackage{amsmath}
\DeclareMathOperator{\arccot}{arccot}
\DeclareMathOperator{\arcsec}{arcsec}
\DeclareMathOperator{\arccsc}{arccsc}
\DeclareMathOperator{\sech}{sech}
\DeclareMathOperator{\csch}{csch}
\DeclareMathOperator{\arcsinh}{arcsinh}
\DeclareMathOperator{\arccosh}{arccosh}
\DeclareMathOperator{\arctanh}{arctanh}
\DeclareMathOperator{\arccoth}{arccoth}
\DeclareMathOperator{\arcsech}{arcsech}
\DeclareMathOperator{\arccsch}{arccsch}
\begin{document}

\begin{equation*}\lim_{x\to0}\frac{\sin x}{x}=1\end{equation*}
\begin{equation*}\lim_{x\to0}\frac{\cos x-1}{x}=0\end{equation*}
\begin{equation*}e^{i\theta}=\cos{\theta}+i\sin{theta}\end{equation*}
\begin{equation*}
e^{i(a+b)}
=\cos(a+b)+i\sin(a+b)
=e^{ia}e^{ib}
=(\cos a+i\sin a)(\cos b+i\sin b)
=\cos a\cos b-\sin a\sin b+i(\cos a\sin b+\sin a\cos b)
\end{equation*}
\begin{equation*}\cos(a+b)=\cos a\cos b-\sin a\sin b\end{equation*}
\begin{equation*}\sin(a+b)=\cos a\sin b+\cos b\sin a\end{equation*}
\begin{equation*}
\frac{d\,f^{-1}(x)}{dx}=\frac{1}{f^\prime(f^{-1}(x))}
\end{equation*}
\hrule
\begin{equation*}
\sin^\prime x
=\lim_{h\to0}\frac{\sin(x+h)-\sin x}{h}
=\lim_{h\to0}\frac{\cos x\sin h+\sin x\cos h-\sin x}{h}
=\lim_{h\to0}\frac{\cos x\sin h+\sin x(\cos h-1)}{h}
=\cos x\left(\lim_{h\to0}\frac{\sin h}{h}\right)+\sin x\left(\lim_{h\to0}\frac{\cos h-1}{h}\right)
=\cos x
\end{equation*}
\hrule
\begin{equation*}
\cos^\prime x
=\frac{d\sqrt{1-\sin^2 x}}{dx}
=\frac{1}{2\sqrt{\sin^2 x-1}}(-1)2\sin x\cos x
=-\frac{2\sin x\cos x}{2\cos x}
=-\sin x
\end{equation*}
\hrule
\begin{equation*}
\tan^\prime x
=\frac{d\frac{\sin x}{\cos x}}{dx}
=\frac{\sin^\prime x\cos x-\sin x\cos^\prime x}{\cos^2 x}
=\frac{\cos x\cos x+\sin x\sin x}{\cos^2 x}
=\frac{\cos^2 x+\sin^2 x}{\cos^2 x}
=\frac{1}{\cos^2 x}
=\sec^2 x
\end{equation*}
\hrule
\begin{equation*}
\cot^\prime x
=\frac{d\frac{1}{\tan x}}{dx}
=-\frac{\tan^\prime x}{\tan^2 x}
=-\frac{\sec^2 x}{\tan^2 x}
=-\frac{1}{\cos^2 x}\frac{\cos^2 x}{\sin^2 x}
=-\frac{1}{\sin^2 x}
=-\csc^2 x
\end{equation*}
\hrule
\begin{equation*}
\sec^\prime x
=\frac{d\frac{1}{\cos x}}{dx}
=-\frac{\cos^\prime x}{\cos^2 x}
=\frac{\sin x}{\cos^2 x}
=\sec x\tan x
\end{equation*}
\hrule
\begin{equation*}
\csc^\prime x
=\frac{d\frac{1}{\sin x}}{dx}
=-\frac{\sin^\prime x}{\sin^2 x}
=-\frac{\cos x}{\sin^2 x}
=-\csc x\cot x
\end{equation*}
\hrule%arsin'
\begin{equation*}
\arcsin^\prime x
=\frac{1}{\sin^\prime(\arcsin(x))}
=\frac{1}{\cos(\arcsin(x))}
\end{equation*}
\begin{equation*}
\Rightarrow\arcsin^\prime (\sin x)
=\frac{1}{\cos(\arcsin(\sin x))}
=\frac{1}{\cos x}
=\frac{1}{\sqrt{1-(\sin x)^2}}
\end{equation*}
\begin{equation*}
\Rightarrow\arcsin^\prime x
=\frac{1}{\sqrt{1-x^2}}
\end{equation*}
\hrule%arccos'
\begin{equation*}
\arccos^\prime x
=\frac{1}{\cos^\prime(\arccos(x))}
=-\frac{1}{\sin(\arccos(x))}
\end{equation*}
\begin{equation*}
\Rightarrow\arccos^\prime (\cos x)
=-\frac{1}{\sin(\arccos(\cos x))}
=-\frac{1}{\sin x}
=-\frac{1}{\sqrt{1-(\cos x)^2}}
\end{equation*}
\begin{equation*}
\Rightarrow\arccos^\prime x
=-\frac{1}{\sqrt{1-x^2}}
\end{equation*}
\hrule%arctan'
\begin{equation*}
\arctan^\prime x
=\frac{1}{\tan^\prime(\arctan(x))}
=\frac{1}{\sec^2(\arctan(x))}
=\cos^2(\arctan x)
\end{equation*}
\begin{equation*}
\Rightarrow\arctan^\prime (\tan x)
=\cos^2(\arctan (\tan x))
=\cos^2 x
\end{equation*}
\begin{equation*}
\tan x
=\frac{\sin x}{\cos x}
=\frac{\sqrt{1-\cos^2 x}}{\cos x}
\end{equation*}
\begin{equation*}\Rightarrow\tan^2 x=\frac{1-\cos^2 x}{\cos^2 x}\end{equation*}
\begin{equation*}\Rightarrow\cos^2 x\tan^2 x=1-\cos^2 x\end{equation*}
\begin{equation*}\Rightarrow\cos^2 x\tan^2 x+\cos^2 x=1\end{equation*}
\begin{equation*}\Rightarrow\cos^2 x(1+\tan^2 x)=1\end{equation*}
\begin{equation*}\Rightarrow\cos^2 x=\frac{1}{1+\tan^2 x}\end{equation*}
\begin{equation*}
\Rightarrow\arctan^\prime (\tan x)
=\cos^2 x
=\frac{1}{1+\tan^2 x}
\end{equation*}
\begin{equation*}
\Rightarrow\arctan^\prime x
=\frac{1}{1+x^2}
\end{equation*}
\hrule%arccot'
\begin{equation*}
\arccot^\prime x
=\frac{1}{\cot^\prime(\arccot(x))}
=-\frac{1}{\csc^2(\arccot(x))}
=-\sin^2(\arccot(x))
\end{equation*}
\begin{equation*}
\Rightarrow\arccot^\prime(\cot x)
=-\sin^2(\arccot(\cot x))
=-\sin^2(x)
\end{equation*}
\begin{equation*}
\cot x
=\frac{\cos x}{\sin x}
=\frac{\sqrt{1-\sin^2 x}}{\sin x}
\end{equation*}
\begin{equation*}
\Rightarrow\cot^2 x
=\frac{1-\sin^2 x}{\sin^2 x}
\end{equation*}
\begin{equation*}
\Rightarrow-\sin^2 x
=-\frac{1}{\cot^2 x+1}
\end{equation*}
\begin{equation*}
\Rightarrow\arccot^\prime(\cot x)
=-\sin^2(x)
=-\frac{1}{\cot^2 x+1}
\end{equation*}
\begin{equation*}
\Rightarrow\arccot^\prime x
=-\frac{1}{x^2+1}
\end{equation*}
\hrule%arcsec'
\begin{equation*}
\arcsec^\prime x
=\frac{1}{\sec^\prime(\arcsec(x))}
=\frac{1}{\sec(\arcsec(x))\tan(\arcsec(x))}
\end{equation*}
\begin{equation*}
\Rightarrow\arcsec^\prime(\sec x)
=\frac{1}{\sec(\arcsec(\sec x))\tan(\arcsec(\sec x))}
=\frac{1}{\sec x\tan x}
\end{equation*}
\begin{equation*}
\tan x
=\frac{\sin x}{\cos x}
=\sec x\sin x
=\sec x\sqrt{1-\cos^2 x}
=\sec x\sqrt{1-\frac{1}{\sec^2 x}}
\end{equation*}
\begin{equation*}
\Rightarrow\tan^2 x
=\sec^2 x\left(1-\frac{1}{\sec^2 x}\right)
=\sec^2 x-1
\end{equation*}
\begin{equation*}
\Rightarrow|\tan x|
=\sqrt{\sec^2 x-1}
\end{equation*}
\begin{equation*}
\Rightarrow\arcsec^\prime(\sec x)
=\frac{1}{\sec x\tan x}
=\frac{1}{|\sec x|\sqrt{\sec^2 x-1}}
\end{equation*}
\begin{equation*}
\Rightarrow\arcsec^\prime(x)
=\frac{1}{|x|\sqrt{x^2-1}}
\end{equation*}
\hrule%arccsc'
\begin{equation*}
\arccsc^\prime x
=\frac{1}{\csc^\prime(\arccsc(x))}
=-\frac{1}{\csc(\arccsc(x))\cot(\arccsc(x))}
\end{equation*}
\begin{equation*}
\Rightarrow\arccsc^\prime (\csc x)
=-\frac{1}{\csc(\arccsc(\csc x))\cot(\arccsc(\csc x))}
=-\frac{1}{\csc x\cot x}
\end{equation*}
\begin{equation*}
\cot x
=\frac{\cos x}{\sin x}
=\frac{\sqrt{1-\sin^2 x}}{\sin x}
=\csc x\sqrt{1-\frac{1}{\csc^2 x}}
\end{equation*}
\begin{equation*}
\Rightarrow\cot^2 x
=\csc^2 x\left(1-\frac{1}{\csc^2 x}\right)
=1-\csc^2 x
\end{equation*}
\begin{equation*}
\Rightarrow|\cot x|
=\sqrt{1-\csc^2 x}
\end{equation*}
\begin{equation*}
\Rightarrow\arccsc^\prime (\csc x)
=-\frac{1}{\csc x\cot x}
=-\frac{1}{|\csc x|\sqrt{1-\csc^2 x}}
\end{equation*}
\begin{equation*}
\Rightarrow\arccsc^\prime x
=-\frac{1}{|x|\sqrt{1-x^2}}
\end{equation*}
\hrule
\begin{equation*}
\sinh x=\frac{e^x-e^{-x}}{2}
\end{equation*}
\hrule
\begin{equation*}
\cosh x=\frac{e^x+e^{-x}}{2}
\end{equation*}
\hrule
\begin{equation*}
\tanh x=\frac{\sinh x}{\cosh x}=\frac{e^x-e^{-x}}{e^x+e^{-x}}
\end{equation*}
\hrule
\begin{equation*}
\coth x=\frac{1}{\tanh x}=\frac{e^x+e^{-x}}{e^x-e^{-x}}
\end{equation*}
\hrule
\begin{equation*}
\sech x=\frac{1}{\cosh x}=\frac{2}{e^x+e^{-x}}
\end{equation*}
\hrule
\begin{equation*}
\csch x=\frac{1}{\sinh x}=\frac{2}{e^x-e^{-x}}
\end{equation*}
\hrule
\begin{equation*}
\arcsinh x=\sinh^{-1} x
\end{equation*}
\hrule
\begin{equation*}
\arccosh x=\cosh^{-1} x
\end{equation*}
\hrule
\begin{equation*}
\arctanh x=\tanh^{-1} x
\end{equation*}
\hrule
\begin{equation*}
\arccoth x=\coth^{-1} x
\end{equation*}
\hrule
\begin{equation*}
\arcsech x=\sech^{-1} x
\end{equation*}
\hrule
\begin{equation*}
\arccsch x=\csch^{-1} x
\end{equation*}
\hrule
\begin{equation*}
\sinh^\prime x
=\frac{d\frac{e^x-e^{-x}}{2}}{dx}
=\frac{e^x+e^{-x}}{2}
=\cosh x
\end{equation*}
\hrule
\begin{equation*}
\cosh^\prime x
=\frac{d\frac{e^x+e^{-x}}{2}}{dx}
=\frac{e^x-e^{-x}}{2}
=\sin x
\end{equation*}
\hrule
\begin{equation*}
\tanh^\prime x
=\frac{d\frac{\sinh x}{\cosh x}}{dx}
=\frac{\sinh^\prime x\cosh x-\sinh x\cosh^\prime x}{\cosh^2 x}
=\frac{\cosh^2 x-\sinh^2 x}{\cosh^2 x}
=\frac{1}{\cosh^2 x}
=\sech^2 x
\end{equation*}
\hrule
\begin{equation*}
\coth^\prime x
=\frac{d\frac{1}{\tanh x}}{dx}
=-\frac{\tanh^\prime x}{\tanh^2 x}
=-\frac{\sech^2 x}{\tanh^2 x}
=-\frac{1}{\cosh^2 x}\frac{\cosh^2 x}{\sinh^2 x}=-\csch^2 x
\end{equation*}
\hrule
\begin{equation*}
\sech^\prime x
=\frac{d\frac{1}{\cosh x}}{dx}
=-\frac{\cosh^\prime x}{\cosh^2 x}
=-\frac{\sinh x}{\cosh^2 x}
=-\sech x\tanh x
\end{equation*}
\hrule
\begin{equation*}
\csch^\prime x
=\frac{d\frac{1}{\sinh x}}{dx}
=-\frac{\sinh^\prime x}{\sinh^2 x}
=-\frac{\cosh x}{\sinh^2 x}
=-\csch x\coth x
\end{equation*}
\hrule
\begin{equation*}
\arcsinh^\prime x
=\frac{1}{\sinh^\prime(\arcsinh x)}
=\frac{1}{\cosh(\arcsinh x)}
\end{equation*}
\begin{equation*}
\Rightarrow\arcsinh^\prime (\sinh x)
=\frac{1}{\cosh(\arcsinh(\sinh x))}
=\frac{1}{\cosh x}
\end{equation*}
\begin{equation*}
\cosh^2 x-\sinh^2 x=1
\end{equation*}
\begin{equation*}
\Rightarrow|\cosh x|=\sqrt{1+\sinh^2 x}
\end{equation*}
\begin{equation*}
\Rightarrow\cosh x=\sqrt{1+\sinh^2 x}
\end{equation*}
\begin{equation*}
\Rightarrow\arcsinh^\prime (\sinh x)
=\frac{1}{\cosh x}
=\frac{1}{\sqrt{1+\sinh^2 x}}
\end{equation*}
\begin{equation*}
\Rightarrow\arcsinh^\prime x
=\frac{1}{\sqrt{1+x^2}}
\end{equation*}
\hrule
\begin{equation*}
\arccosh^\prime x
=\frac{1}{\cosh^\prime(\arccosh x)}
=\frac{1}{\sinh(\arcsinh x)}
\end{equation*}
\begin{equation*}
\Rightarrow\arccosh^\prime (\cosh x)
=\frac{1}{\sinh(\arccosh(\cosh x))}
=\frac{1}{\sinh x}
\end{equation*}
\begin{equation*}
\cosh^2 x-\sinh^2 x=1
\end{equation*}
\begin{equation*}
\Rightarrow|\sinh x|=\sqrt{\cosh^2 x-1}
\end{equation*}
\begin{equation*}
\Rightarrow\sinh x=\sqrt{\cosh^2 x-1}
\end{equation*}
\begin{equation*}
\Rightarrow\arccosh^\prime (\cosh x)
=\frac{1}{\sinh x}
=\frac{1}{\sqrt{\cosh^2 x-1}}
\end{equation*}
\begin{equation*}
\Rightarrow\arccosh^\prime x
=\frac{1}{\sqrt{x^2-1}}
\end{equation*}
\hrule
\begin{equation*}
\arctanh^\prime x
=\frac{1}{\tanh^\prime(\arctanh x)}
=\frac{1}{\sech^2(\arctanh x)}
\end{equation*}
\begin{equation*}
\Rightarrow\arctanh^\prime(\tanh x)
=\frac{1}{\sech^2(\arctanh(\tanh x))}
=\frac{1}{\sech^2 x}
\end{equation*}
\begin{equation*}
\tanh^2 x
=\frac{\sinh^2 x}{\cosh^2 x}
=\sech^2 x \sinh^2 x
=\sech^2 x (\cosh^2 x-1)
=\sech^2 x \left(\frac{1}{\sech^2 x}-1\right)
=1-\sech^2 x
\end{equation*}
\begin{equation*}
\Rightarrow\sech^2 x
=1-\tanh^2 x
\end{equation*}
\begin{equation*}
\Rightarrow\arctanh^\prime(\tanh x)
=\frac{1}{1-\tanh^2 x}
\end{equation*}
\begin{equation*}
\Rightarrow\arctanh^\prime x
=\frac{1}{1-x^2}
\end{equation*}
\hrule
\begin{equation*}
\arccoth^\prime x
=\frac{1}{\coth^\prime(\arccoth x)}
=-\frac{1}{\csch^2(\arccoth x)}
\end{equation*}
\begin{equation*}
\Rightarrow\arccoth^\prime(\coth x)
=-\frac{1}{\csch^2(\arccoth(\coth x))}
=-\frac{1}{\csch^2 x}
\end{equation*}
\begin{equation*}
\coth x
=\frac{\cosh x}{\sinh x}
=\csch x\cosh x
=\csch x\sqrt{1+\sinh^2 x}
=\csch x\sqrt{1+\frac{1}{\csch^2 x}}
\end{equation*}
\begin{equation*}
\Rightarrow\coth^2 x
=\csch^2 x\left(1+\frac{1}{\csch^2 x}\right)
=\csch^2 x+1
\end{equation*}
\begin{equation*}
\Rightarrow\csch^2 x
=\coth^2 x-1
\end{equation*}
\begin{equation*}
\Rightarrow\arccoth^\prime(\coth x)
=-\frac{1}{\csch^2 x}
=-\frac{1}{\coth^2 x-1}
\end{equation*}
\begin{equation*}
\Rightarrow\arccoth^\prime x
=-\frac{1}{\csch^2 x}
=-\frac{1}{x^2-1}
\end{equation*}
\hrule
\begin{equation*}
\arcsech^\prime x
=\frac{1}{\sech^\prime(\arcsech x)}
=-\frac{1}{\sech(\arcsech x)\tanh(\arcsech x)}
\end{equation*}
\begin{equation*}
\Rightarrow\arcsech^\prime(\sech x)
=-\frac{1}{\sech(\arcsech(\sech x))\tanh(\arcsech (\sech x))}
=-\frac{1}{\sech x\tanh x}
\end{equation*}
\begin{equation*}
\tanh x
=\frac{\sinh x}{\cosh x}
=\sech x\sinh x
=\sech x\sqrt{\cosh^2 x-1}
=\sech x\sqrt{\frac{1}{\sech^2 x}-1}
=\sqrt{1-\sech^2 x}
\end{equation*}
\begin{equation*}
\Rightarrow\arcsech^\prime(\sech x)
=-\frac{1}{\sech x\tanh x}
=-\frac{1}{\sech x\sqrt{1-\sech^2 x}}
\end{equation*}
\begin{equation*}
\Rightarrow\arcsech^\prime x
=-\frac{1}{\sech x\tanh x}
=-\frac{1}{x\sqrt{1-x^2}}
\end{equation*}
\hrule
\begin{equation*}
\arccsch^\prime x
=\frac{1}{\csch^\prime(\arccsch x)}
=-\frac{1}{\csch(\arccsch x)\coth(\arccsch x)}
\end{equation*}
\begin{equation*}
\Rightarrow\arccsch^\prime(\csch x)
=-\frac{1}{\csch(\arccsch(\csch x))\coth(\arccsch(\csch x))}
=-\frac{1}{\csch x\coth x}
\end{equation*}
\begin{equation*}
\coth x
=\frac{\cosh x}{\sinh x}
=\csch x\cosh x
=\csch x\sqrt{1+\sinh^2 x}
=\csch x\sqrt{1+\frac{1}{\csch^2 x}}
=\sqrt{\csch^2 x+1}
\end{equation*}
\begin{equation*}
\Rightarrow\arccsch^\prime(\csch x)
=-\frac{1}{\csch x\coth x}
=-\frac{1}{\csch x\sqrt{\csch^2 x+1}}
\end{equation*}
\begin{equation*}
\Rightarrow\arccsch^\prime x
=-\frac{1}{x\sqrt{x^2+1}}
\end{equation*}
\end{document}
